# Билет №14
Площадь многоугольной фигуры. Формулы площади треугольника.

## Герон
[![Герон](geron-geogebra.png)](https://www.geogebra.org/geometry/n8hshfws)

Запишем теорему Пифагора:

<<<<<<< HEAD
$$ h^2 = c^2 - x^2 = a^2 - (b - x)^2; \\
(b - 2x)b = a^2 - c^2; \\
b - 2x = \frac{a^2 - c^2}{b}; \\
=======
$$ h^2 = c^2 - x^2 = a^2 - (b - x)^2; \newline
(b - 2x)b = a^2 - c^2; \newline
b - 2x = \frac{a^2 - c^2}{b}; \newline
>>>>>>> c9fabb6979dc1ebf7eb65b1cc3953a50dc723445
x = \frac{b^2 - a^2 + c^2}{2b} $$

Распишем то выражение:

$$ h^2 = c^2 - x^2 = c^2 - (\frac{b^2 - a^2 + c^2}{2b})^2 = \newline
= \frac{2bc - b^2 + a^2 - c^2}{2b} \cdot \frac{2bc + b^2 - a^2 + c^2}{2b} = \newline
= \frac{a^2 - (b - c)^2}{2b} \cdot \frac{(b + c)^2 - a^2}{2b} = \newline
= \frac{(a + c - b)(a + b - c)(a + b + c)(b + c - a)}{(2b)^2} = \newline
= \frac{2^4 \cdot p(p - a)(p - b)(p - c)}{4b^2} = \frac{4 \cdot p(p - a)(p - b)(p - c)}{b^2} \Rightarrow \newline
\Rightarrow h = 2 \cdot \frac{\sqrt{p(p - a)(p - b)(p - c)}}{b} \Rightarrow \newline
\Rightarrow S = \frac{b \cdot h}{2} = \sqrt{p(p - a)(p - b)(p - c)} $$






{% include lib/mathjax.html %}
